Distributed.lean
@@ -1,1 +1,2 @@
-import Distributed.paper_proofs
+import Distributed.Paper.paper_proofs
+import Distributed.Paxos.main
