Distributed/Paxos/acceptors.lean
@@ -1,0 +1,10 @@
+import Distributed.base_structures
+import Distributed.Paxos.paxos_model
+import Mathlib.Tactic.ByContra
+import Mathlib.Tactic.Cases 
+
+open Model
+open PaxosModel
+namespace PaxosProof
+
+
