Distributed/Paxos/learner_helpers.lean
@@ -1,0 +1,207 @@
+import Distributed.base_structures
+import Distributed.Paxos.paxos_model
+import Mathlib.Tactic.ByContra
+import Mathlib.Tactic.Cases 
+
+open Model
+open PaxosModel
+namespace PaxosProof
+
+def inv43 (s1: System a l p) (i: Fin a) (v: Value) (id: PropId):=
+(s1.acceptors i).accepted = some (v, id)
+-> (s1.acceptors i).maxPrepareId >= id
+
+
+theorem inv43Proof_ind (s1 s2: System a l p) (i: Fin a)  (v: Value) (id: PropId) :
+step s1 s2
+-> inv43 s1 i v id
+-> (∀ i, (s1.acceptors i).id = i)
+-> inv43 s2 i v id := by
+simp [inv43]; intros step IH kIsTrue learnInN
+cases step <;> rename_i stepRule <;> cases stepRule <;> (try (rename_i stepRule; simp at stepRule; grind)) <;> (try (simp [updateMap] at *; split <;> try grind  ))
+. rename_i j pid mess acc net stepRule eq; subst eq
+  split at learnInN <;> try grind
+  rcases stepRule with ⟨ messRules, accNat, netNat⟩; subst accNat 
+  simp at ⊢ learnInN; have b1 := IH learnInN; have b2 := messRules.right.right
+  exact Nat.le_of_lt (Nat.lt_of_le_of_lt b1 b2)
+. rename_i stepRule eq; split at learnInN <;> try grind
+  rcases stepRule with ⟨ messAcc, b2, mInN, accNat⟩; subst eq; subst accNat
+  simp at ⊢ learnInN; simp [learnInN, PropId]
+
+
+theorem inv43Proof (s: System a l p) (v: Value) (i: Fin a) (id: PropId)  :
+systemIsValid s
+-> inv43 s i v id:= by
+intros sIsValid
+have ⟨ s0, s0Inits, s0Steps ⟩ := sIsValid
+induction s0Steps  with
+| refl =>
+  simp [systemInits, acceptorInits] at s0Inits
+  simp [inv43, s0Inits] at ⊢
+| trans s2 s3 s0Steps s2Step IH=>
+  simp [systemIsValid, ] at (IH)
+  have IHApp := IH s0; simp [s0Inits, s0Steps] at IHApp
+  have s2Valid:(systemIsValid s2) := by (simp [systemIsValid]; grind)
+  --have IH2 := inv43Proof s2 v i id s2Valid
+  exact (inv43Proof_ind s2 s3 i v id s2Step IHApp (idIsK s2 s2Valid))
+
+
+def inv42 (s1: System a l p) (i: Fin a) (v: Value) (id: PropId):=
+Message.Learn (i, v, id) ∈ s1.network.messages
+-> (s1.acceptors i).maxPrepareId >= id
+
+
+
+theorem inv42Proof_ind (s1 s2: System a l p) (i: Fin a)  (v: Value) (id: PropId) :
+step s1 s2
+-> inv42 s1 i v id
+-> (∀ i, (s1.acceptors i).id = i)
+-> inv43 s1 i v id
+-> inv42 s2 i v id := by
+simp [inv42]; intros step IH kIsTrue i43  learnInN
+cases step <;> rename_i stepRule <;> cases stepRule <;> (try (rename_i stepRule; simp at stepRule; grind)) <;> (try (simp [updateMap] at *; split <;> try grind  ))
+. rename_i j pid mess acc net  stepRule eq;
+  rcases stepRule with ⟨ mRules, accNat, natRules ⟩ 
+  subst_vars; simp; rw [natRules] at learnInN; simp at learnInN
+  have IHApp := IH learnInN
+  exact Nat.le_of_lt (Nat.lt_of_le_of_lt  IHApp mRules.right.right)
+. have IHApp := IH learnInN; rename_i stepRule eq
+  rcases stepRule with ⟨ mNat, idBound, mInN, a2Nat ⟩; subst a2Nat ; simp; subst eq
+  exact (Nat.le_trans  IHApp idBound)
+. rename_i j net v' pid stepRule
+  rcases stepRule with ⟨ accIsSome , netNat ⟩ ; rw [netNat] at learnInN
+  simp at learnInN; cases learnInN <;> try grind
+  rename_i eq; rcases eq with ⟨ eq1, eq2, eq3 ⟩;
+  subst_vars; rw [kIsTrue j] at *
+  simp at *; have bound :=  i43 accIsSome
+  simp [bound]
+
+theorem inv42Proof (s: System a l p) (v: Value) (i: Fin a) (id: PropId)  :
+systemIsValid s
+-> inv42 s i v id:= by
+intros sIsValid
+have ⟨ s0, s0Inits, s0Steps ⟩ := sIsValid
+induction s0Steps  with
+| refl =>
+  simp [systemInits, networkInits] at s0Inits
+  simp [inv42, s0Inits] at ⊢
+| trans s2 s3 s0Steps s2Step IH=>
+  simp [systemIsValid, ] at (IH)
+  have IHApp := IH s0; simp [s0Inits, s0Steps] at IHApp
+  have s2Valid:(systemIsValid s2) := by (simp [systemIsValid]; grind)
+  have IH2 := inv43Proof s2 v i id s2Valid
+  exact (inv42Proof_ind s2 s3 i v id s2Step IHApp (idIsK s2 s2Valid) IH2)
+
+
+-- INV41
+def inv41 (s1: System a l p) (i: Fin a) (v: Value) (id: PropId):=
+Message.Learn (i, v, id) ∈ s1.network.messages
+-> ∃ v' id', id' >= id ∧ (s1.acceptors i).accepted = some (v', id')
+
+theorem inv41Proof_ind (s1 s2: System a l p) (i: Fin a)  (v: Value) (id: PropId) :
+step s1 s2
+-> inv41 s1 i v id
+-> (∀ i, (s1.acceptors i).id = i)
+-> inv42 s1 i v id
+-> inv41 s2 i v id := by
+simp [inv41]; intros step IH iBound i42 learnInN
+cases step <;> rename_i stepRule <;> cases stepRule <;> try (rename_i stepRule; simp at stepRule; grind)
+. rename_i j pid mess acc net stepRule
+  simp [updateMap] at *
+  split <;> try grind  
+. rename_i pid j v' acc mess stepRule
+  simp [updateMap] at *
+  split <;> try grind
+  rcases stepRule with ⟨ mNat, mIdBound, mInN, accNat ⟩; subst accNat
+  simp;
+  have dd := i42 learnInN; rename_i eq; subst eq
+  exact (Nat.le_trans dd mIdBound)
+. rename_i j net v' pid stepRule
+  rcases stepRule with ⟨ sAcc, nNat ⟩; simp at learnInN;rw [nNat] at learnInN; simp at ⊢ learnInN
+  cases learnInN <;> try grind
+  rename_i eqs; rcases eqs with ⟨ iId, vEq, idEq ⟩; subst_vars
+  exists v'; exists pid; simp [PropId, iBound]; exact sAcc
+
+
+theorem inv41Proof (s: System a l p) (v: Value) (i: Fin a) (id: PropId)  :
+systemIsValid s
+-> inv41 s i v id:= by
+intros sIsValid
+have ⟨ s0, s0Inits, s0Steps ⟩ := sIsValid
+induction s0Steps  with
+| refl =>
+  simp [systemInits, networkInits] at s0Inits
+  simp [inv41, s0Inits] at ⊢
+| trans s2 s3 s0Steps s2Step IH=>
+  simp [systemIsValid, ] at (IH)
+  have IHApp := IH s0; simp [s0Inits, s0Steps] at IHApp
+  have s2Valid:(systemIsValid s2) := by (simp [systemIsValid]; grind)
+  have IH2 := inv42Proof s2 v i id s2Valid
+  exact (inv41Proof_ind s2 s3 i v id s2Step IHApp (idIsK s2 s2Valid) IH2)
+
+def inv31 (s1: System a l p) (i: Fin a) (v: Value) (id: PropId):=
+(s1.acceptors i).accepted = some (v, id)
+->  Message.Accept (id, v) ∈ s1.network.messages
+
+theorem inv31Proof_ind (s1 s2: System a l p) (i: Fin a) (v: Value) (id: PropId) :
+step s1 s2
+-> inv31 s1 i v id
+-> inv31 s2 i v id := by
+simp [inv31]; intros step  IH accIsSome
+cases step <;> rename_i stepRule <;> cases stepRule <;> try (rename_i stepRule; simp at stepRule; grind)
+. rename_i j pid m acc n stepRule; simp [updateMap] at *
+  split at accIsSome <;> try grind
+. rename_i pid j v' acc m stepRule; simp [updateMap] at *
+  split at accIsSome <;> try grind
+
+
+theorem inv31Proof (s: System a l p) (i: Fin a) (v: Value) (id: PropId) :
+systemIsValid s
+-> inv31 s i v id := by
+intros sIsValid 
+rcases sIsValid with ⟨ s0, s0Inits, s0Steps ⟩
+induction s0Steps  with
+| refl =>
+  simp [systemInits, acceptorInits] at s0Inits
+  simp [inv31, s0Inits] at ⊢ 
+| trans s2 s3 s0Steps s2Step IH=>
+  exact (inv31Proof_ind s2 s3 i v id s2Step IH)
+
+
+
+def inv3 (s1: System a l p) (i: Fin a) (v: Value) (id: PropId):=
+Message.Learn (i, v, id) ∈ s1.network.messages
+->  Message.Accept (id, v) ∈ s1.network.messages
+theorem inv3Proof_ind (s1 s2: System a l p) (i: Fin a) (v: Value) (id:PropId) :
+step s1 s2
+-> inv3 s1 i v id
+-> (∀ i, (s1.acceptors i).id = i)
+-> inv31 s1 i v id
+-> inv3 s2 i v id := by
+simp [inv3, inv31]; intros step  IH accIsK IH2 sIsSome
+cases step <;> rename_i stepRule <;> cases stepRule <;> try (rename_i stepRule; simp at stepRule; grind)
+
+
+
+
+theorem inv3Proof (s: System a l p) (i: Fin a) (v: Value) (id: PropId) :
+systemIsValid s
+-> inv3 s i v id := by
+intros sIsValid
+have ⟨ s0, s0Inits, s0Steps ⟩ := sIsValid
+induction s0Steps  with
+| refl =>
+  simp [systemInits, networkInits] at s0Inits
+  simp [inv3, s0Inits] at ⊢ 
+| trans s2 s3 s0Steps s2Step IH=>
+  simp [systemIsValid, ] at (IH)
+  have IHApp := IH s0; simp [s0Inits, s0Steps] at IHApp
+  have s2Valid:(systemIsValid s2) := by (simp [systemIsValid]; grind)
+  have IH2 := inv31Proof s2 i v id s2Valid
+  exact (inv3Proof_ind s2 s3 i v id s2Step IHApp (idIsK s2 s2Valid) IH2)
+
+
+def inv5 (s: System a l p) (i: Fin p)(id: PropId) (v: Value):=
+Message.Accept (id, v) ∈ s.network.messages
+-> (s.proposers i).propVal = some v
+-> id <= (s.proposers i).propId
