Distributed/Paxos/p2a.lean
@@ -1,0 +1,60 @@
+import Distributed.base_structures
+import Distributed.Paxos.paxos_model
+import Distributed.Paxos.p2b
+import Mathlib.Tactic.ByContra
+import Mathlib.Tactic.Cases 
+
+open Model
+open PaxosModel
+namespace PaxosProof
+
+def inv4a1 (s: System a l p) (i: Fin a) (v : Value) (id: PropId) :=
+(s.acceptors i).accepted = some (v, id)
+-> Message.Accept (id, v) ∈ s.network.messages
+
+
+
+theorem inv4a1Proof_ind (s1 s2: System a l p) (i: Fin a) (v: Value) (id: PropId) :
+step s1 s2
+-> inv4a1 s1 i v id
+-> inv4a1 s2 i v id := by
+simp [inv4a1]; intros step IH sIsSome 
+cases step <;> rename_i stepRule <;> cases stepRule <;> (try (rename_i stepRule; simp at stepRule; grind))
+. rename_i j pid mess acc net stepRule
+  rcases stepRule with ⟨mRules, accNat, netNat⟩; subst accNat
+  simp; rw [netNat]; simp; clear netNat; simp [updateMap] at sIsSome; split at sIsSome <;> try grind  
+. rename_i pid j v' acc mess stepRule
+  simp [updateMap] at ⊢ sIsSome; split at sIsSome <;> try grind
+  rcases stepRule with ⟨ mAcc, accBound, mInN, accNat⟩; subst accNat mAcc
+  simp at sIsSome; rcases sIsSome with ⟨ eq1, eq2 ⟩; subst eq1 eq2
+  exact mInN
+
+
+
+theorem inv4a1Proof (s: System a l p) (i: Fin a) (v: Value) (id: PropId)  :
+systemIsValid s
+-> inv4a1 s i v id:= by 
+intros sIsValid 
+rcases sIsValid with ⟨ s0, s0Inits, s0Steps ⟩
+induction s0Steps  with
+| refl =>
+  simp [systemInits, acceptorInits] at s0Inits
+  simp [inv4a1, s0Inits] at ⊢ 
+| trans s2 s3 s0Steps s2Step IH=>
+  exact (inv4a1Proof_ind s2 s3 i v id s2Step IH)
+
+
+
+-- INV4a: learners and an accepted element show that there is 
+def inv4a (s: System a l p) (v : Value) (id: PropId) :=
+(∃ set, count set > a / 2 ∧ (∀ (i: Fin a), contains  set i -> Message.Learn (i, v, id) ∈ s.network.messages))
+-> ∀ id' i v', (s.acceptors i).accepted = some (v', id')
+->  id' >= id
+->  v = v'
+
+theorem inv4aProof (s: System a l p) (v: Value) (id: PropId)  :
+systemIsValid s
+-> inv4a s v id:= by
+intros sIsValid set id1 i v' accIn idBound
+have p2 := inv4a1Proof s i v' id1 sIsValid accIn
+exact (inv4bProof s v id sIsValid set id1 v' p2 idBound)
