Distributed/Paxos/p2b.lean
@@ -1,0 +1,72 @@
+import Distributed.base_structures
+import Distributed.Paxos.paxos_model
+import Distributed.Paxos.p2c
+import Distributed.Paxos.learner_helpers
+import Mathlib.Tactic.ByContra
+import Mathlib.Tactic.Cases 
+
+open Model
+open PaxosModel
+namespace PaxosProof
+
+
+-- INV4b1
+
+def inv4b1 (s: System a l p) (i: Fin a) (v: Value) (id: PropId) :=
+Message.Learn (i,  v, id)  ∈ s.network.messages
+-> ∀  id' p, Message.Promise id' i p ∈ s.network.messages
+-> id' >= id
+-> p ≠ none
+
+
+
+theorem inv4b1Proof_ind (s1 s2: System a l p) (i: Fin a)  (v: Value) (id: PropId) :
+step s1 s2
+-> inv4b1 s1 i v id
+-> inv41  s1 i v id
+-> (∀ i, (s1.acceptors i).id = i)
+-> inv4b1 s2 i v id := by
+   simp [inv4b1]; intros step IH i41 iEq i4b2 mLearn id2 prop  mProp id2Boun
+   sorry
+theorem inv4b1Proof (s: System a l p) (i: Fin a) (v: Value) (id: PropId)  :
+systemIsValid s
+-> inv4b1 s i v id:= by
+intros sIsValid
+have ⟨ s0, s0Inits, s0Steps ⟩ := sIsValid
+induction s0Steps  with
+| refl =>
+  simp [systemInits, networkInits] at s0Inits
+  simp [inv4b1, s0Inits] at ⊢
+| trans s2 s3 s0Steps s2Step IH=>
+  simp [systemIsValid, ] at (IH)
+  have IHApp := IH s0; simp [s0Inits, s0Steps] at IHApp
+  have s2Valid:(systemIsValid s2) := by (simp [systemIsValid]; grind)
+  have p1 := inv41Proof s2 v i id s2Valid
+  sorry
+
+
+-- INV4b
+def inv4b (s: System a l p) (v : Value) (id: PropId) :=
+(∃ set, count set > a / 2 ∧ (∀ (i: Fin a), contains  set i -> Message.Learn (i, v, id) ∈ s.network.messages))
+-> ∀ id' v', Message.Accept (id', v') ∈ s.network.messages
+->  id' >= id
+->  v = v'
+
+
+theorem inv4bProof (s: System a l p) (v: Value) (id: PropId)  :
+systemIsValid s
+-> inv4b s v id:= by
+intros sIsValid setRule id2 v2 mAccs
+rcases setRule with ⟨ set1, setCount1, setContains1 ⟩ 
+have ⟨ set2, setCount2, setContains2R1, setContains2R2 ⟩  := inv4cProof s v2 id2 sIsValid mAccs
+have ⟨ i, iContained1, iContained2 ⟩ := setMaxContainsBoth set1 set2 setCount1 setCount2
+rcases setContains2R2 with setContains2R2 | setContains2R3
+. have p1 := setContains2R2 i iContained2
+  have p2 := setContains1 i iContained1
+  intros id2Bound; exfalso
+  have dd := inv4b1Proof s i v id sIsValid p2 id2 none p1 id2Bound (by simp)
+  exact dd
+. rcases setContains2R3 with ⟨ existsOneId, forAllId ⟩ 
+  have p2 := setContains1 i iContained1
+  have ⟨ prop , p3 ⟩ := setContains2R1 i iContained2
+  sorry
