Distributed/Paxos/p2c.lean
@@ -1,0 +1,182 @@
+import Distributed.base_structures
+import Distributed.Paxos.paxos_model
+import Distributed.Paxos.learner_helpers
+import Mathlib.Tactic.ByContra
+import Mathlib.Tactic.Cases
+
+open Model
+open PaxosModel
+namespace PaxosProof
+
+
+
+def inv4c4 (s: System a l p) (i: Fin p) (j: Fin a) :=
+(s.proposers i).propRec j = true
+-> (Message.Promise (s.proposers i).propId j none ∈ s.network.messages ∨ ∃ v, (s.proposers i).propVal = some v)
+
+
+--INV4c1
+def inv4c1 (s: System a l p) (i: Fin p) :=
+(s.proposers i).propVal = none
+-> ∀ j, contains (s.proposers i).propRec j = true
+-> Message.Promise (s.proposers i).propId j none ∈ s.network.messages
+
+
+theorem inv4c1Proof_ind (s1 s2: System a l p) (i: Fin p):
+step s1 s2
+-> inv4c1 s1 i
+-> inv4c1 s2 i := by
+simp [inv4c1]; intros step IH sPropNone j jContained
+cases step <;> rename_i stepRule <;> cases stepRule <;> repeat (rename_i stepRule; rcases stepRule) <;> (try simp [updateMap] at * <;> split) <;> (try grind)
+. unfold contains emptySet at jContained; grind
+. simp at *; rename_i s; split at s <;> try grind
+  subst_vars; simp at *;
+  simp [insertElem, contains, updateMap] at jContained IH
+  cases jContained <;> try grind
+
+
+theorem inv4c1Proof (s: System a l p) (i: Fin p):
+systemIsValid s
+-> inv4c1 s i:= by
+intros sIsValid 
+rcases sIsValid with ⟨ s0, s0Inits, s0Steps ⟩
+induction s0Steps  with
+| refl =>
+  simp [systemInits, proposerInits, networkInits] at s0Inits
+  simp [inv4c1, s0Inits, ] at ⊢
+  unfold emptySet contains;grind
+| trans s2 s3 s0Steps s2Step IH=>
+  exact (inv4c1Proof_ind s2 s3 i s2Step  IH)
+
+
+
+
+--INV4c2
+def inv4c2 (s: System a l p) (i: Fin p) (v: Value):=
+(s.proposers i).propVal = v
+-> (∃ j, contains (s.proposers i).propRec j = true
+∧ Message.Promise (s.proposers i).propId j (some (v, (s.proposers i).accPropId )) ∈ s.network.messages)
+∧ (∀ j, contains (s.proposers i).propRec j = true
+-> (∃ v' id', (Message.Promise (s.proposers i).propId j (some (v', id')) ∈ s.network.messages ∧   id' <= (s.proposers i).accPropId)) ∨ Message.Promise (s.proposers i).propId j none ∈ s.network.messages)
+
+
+theorem inv4c2Proof_ind (s1 s2: System a l p) (i: Fin p) (v: Value):
+step s1 s2
+-> inv4c2 s1 i v
+-> (∀ j v id, inv43 s1 j v id)
+-> (∀ j, inv4c4 s1 i j)
+-> inv4c2 s2 i v := by
+simp [inv4c2]; intros step IH i43 i4c4 sPropNone 
+cases step <;> rename_i stepRule <;> cases stepRule <;> repeat (rename_i stepRule; rcases stepRule) <;> (try simp [updateMap] at * <;> split) <;> (try grind) <;> subst_vars
+. rename_i j k prop opt v pid2 mInN  idBound splitX
+  simp at *; split at splitX
+  . subst splitX; simp [contains, insertElem, updateMap] at *
+    constructor <;> try grind
+  . rcases splitX with ⟨ eq1, eq2 ⟩; subst eq1 eq2; simp [contains, insertElem, updateMap] at *
+    constructor <;> try grind
+    subst sPropNone; intros h eq
+    cases eq
+    rename_i k; subst k; left; exists v, pid2; constructor <;> try grind
+    simp [PropId]; rename_i acc
+    sorry
+. simp at *; subst_vars; rename_i v net k retBound
+  split at retBound; try grind
+  . clear IH; rw [retBound]; simp
+. sorry
+
+
+theorem inv4c2Proof (s: System a l p) (i: Fin p) (v: Value):
+systemIsValid s
+-> inv4c2 s i v:= by
+intros sIsValid 
+rcases sIsValid with ⟨ s0, s0Inits, s0Steps ⟩
+induction s0Steps  with
+| refl =>
+  simp [systemInits, proposerInits, networkInits] at s0Inits
+  simp [inv4c2, s0Inits, ] at ⊢
+| trans s2 s3 s0Steps s2Step IH=>
+  sorry
+
+--INV4c3
+def inv4c3 (s: System a l p) (j: Fin p) :=
+(s.proposers j).accPropId ≤ (s.proposers j).propId
+
+
+theorem inv4c3Proof_ind (s1 s2: System a l p) (i: Fin p):
+step s1 s2
+-> inv4c3 s1 i 
+-> inv4c3 s2 i := by
+simp [inv4c3]; intros step IH 
+cases step <;> rename_i stepRule <;> cases stepRule <;> repeat (rename_i stepRule; rcases stepRule) <;> (try simp [updateMap] at * <;> split) <;> (try grind)
+. simp [uniqueId]; exact Nat.zero_le _
+
+  
+theorem inv4c3Proof (s: System a l p) (i: Fin p):
+systemIsValid s
+-> inv4c3 s i:= by
+intros sIsValid 
+rcases sIsValid with ⟨ s0, s0Inits, s0Steps ⟩
+induction s0Steps  with
+| refl =>
+  simp [systemInits, proposerInits, networkInits] at s0Inits
+  simp [inv4c3, s0Inits, ] at ⊢;
+  grind
+| trans s2 s3 s0Steps s2Step IH=>
+  exact (inv4c3Proof_ind s2 s3 i s2Step  IH)
+
+
+
+-- INV4c: The message implies there is a set of elements in both places
+def inv4c (s: System a l p) (v : Value) (id: PropId) :=
+Message.Accept (id, v) ∈ s.network.messages
+ -> ∃ (set: Set a), count set > a / 2
+∧ (∀ i, contains set i -> ∃ p, Message.Promise id i p ∈ s.network.messages) 
+∧ ((∀ i, contains set i -> Message.Promise id i none ∈ s.network.messages)
+∨ (∃ idmax, idmax <= id  ∧ ((∃ i, contains set i ∧ Message.Promise  id i (some (v, idmax)) ∈ s.network.messages)
+∧ (∀ i, contains set i  -> ∃ v' id', Message.Promise id i (some (v', id')) ∈ s.network.messages -> id' <= idmax))))
+
+theorem inv4cProof_ind (s1 s2: System a l p) (v: Value) (id: PropId):
+step s1 s2
+-> inv4c s1 v id
+-> (∀ i , inv4c1 s1 i )
+-> (∀ i v, inv4c2 s1 i v)
+-> (∀ i, inv4c3 s1 i)
+-> (∀ i v id, inv43 s1 i v id)
+-> inv4c s2 v id := by
+simp [inv4c]; intros step IH i4c1 i4c2 i4c3 i43 accInN
+cases step <;> rename_i stepRule <;> cases stepRule <;> repeat (rename_i stepRule; rcases stepRule) <;> (try (rename_i mNat; rw [mNat] at accInN ⊢)) <;> (try (simp at accInN ⊢; exact (IH accInN))) <;> try grind
+. simp at accInN mNat; subst_vars; rename_i mNat
+  rw [mNat] at accInN ⊢; simp at accInN ⊢ ; exact (IH accInN)
+. simp at *; clear i4c1 i4c2 i4c3 i43
+  have ⟨ set, setCount, setContains ⟩ := IH accInN
+  exists set; simp [setCount]
+  constructor; have c := setContains.left; grind
+  cases setContains.right
+  . left; grind
+  . right; rename_i c; rcases c with ⟨ idMax, idMaxBound, rest ⟩   
+    exists idMax; simp [idMaxBound];
+    constructor <;> try grind
+    sorry
+. sorry
+. rename_i prop v2 net j propRecCount pNat splitN; simp at accInN ⊢ 
+  split at splitN <;> (try rw [splitN] at accInN ⊢) <;> (try rw [splitN.left] at accInN ⊢) <;> simp at accInN ⊢ <;> cases accInN <;> rename_i accInN <;> (try (exact IH accInN)) <;> exists (s1.proposers j).propRec <;> simp [propRecCount] <;> rename_i eq <;> simp at eq <;> rcases accInN with ⟨ eq1, eq2 ⟩ 
+  . have dd := i4c1 j eq
+    constructor
+    . intros i iContained; exists none; rw [eq1]; exact (dd i iContained)
+    . left; intros i iContained; rw [eq1]; exact (dd  i iContained)
+  .sorry
+    
+    
+    
+
+theorem inv4cProof (s: System a l p) (v: Value) (id: PropId)  :
+systemIsValid s
+-> inv4c s v id:= by
+intros sIsValid 
+rcases sIsValid with ⟨ s0, s0Inits, s0Steps ⟩
+induction s0Steps  with
+| refl =>
+  simp [systemInits, networkInits] at s0Inits
+  simp [inv4c, s0Inits] at ⊢ 
+| trans s2 s3 s0Steps s2Step IH=>
+  sorry
